ReplicatedDisk.v
@@ -1,3 +1,4 @@
+Require Import Automation.
 Require Import DecidableEquality.
 Require Import Prog.
 Require SequentialDisk.
@@ -25,6 +26,13 @@ Proof.
   destruct (is_eq a2 a3); intuition.
 Qed.
 
+Lemma vote_eq : forall A {AEQ:EqDec A} a a',
+    vote a a a' = a.
+Proof.
+  unfold vote; intros.
+  destruct matches.
+Qed.
+
 Definition RRead_impl (a:addr) : prog3 block :=
   v0 <- Read d0 a;
     v1 <- Read d1 a;
@@ -46,3 +54,158 @@ Fixpoint translate T (p: seq_prog T) : prog3 T :=
  | Bind p p' => Prog.Bind (translate p)
                          (fun r => translate (p' r))
  end.
+
+(** We will now show a simulation between the single-disk semantics and
+single-disk programs implemented using replication on top of a 3-disk
+configuration.
+
+The idea of this proof is that correctness of a seq_prog in terms of the
+supposed single-disk semantics should carry over to correctness of the
+translated program (which implements a sequential program using replication).
+The proof will show that from a pair of related states, any behavior of the
+seq_prog can be re-produced as related behavior in the translated prog3.
+ *)
+
+(* The simulation is defined in terms of relating the states of the two
+programs. Our relation captures replicated configurations line up with a
+sequential disk. *)
+Definition sigma_rel (ssigma:SSigma) (sigma:Sigma) : Prop :=
+  forall a, match sdisk ssigma a with
+       | Some v => exists v0 v1 v2,
+                  disk0 sigma a = Some v0 /\
+                  disk1 sigma a = Some v1 /\
+                  disk2 sigma a = Some v2 /\
+                  v = vote v0 v1 v2
+       | None => disk0 sigma a = None /\
+                disk1 sigma a = None /\
+                disk2 sigma a = None
+       end.
+
+Inductive result_rel Sigma1 Sigma2 (rel: Sigma1 -> Sigma2 -> Prop) T :
+  Result Sigma1 T -> Result Sigma2 T -> Prop :=
+| Finished_rel : forall sigma1 sigma2 v,
+    rel sigma1 sigma2 ->
+    result_rel rel (Finished v sigma1) (Finished v sigma2)
+(* there is one more valid simulation: if the first relation succeeds, then it's
+   ok for the second to fail, in the order Sigma1 and Sigma2 are given here. *)
+| Crashed_rel : forall sigma1 sigma2,
+    rel sigma1 sigma2 ->
+    (* this is too strong: should be able to state any relation for crash states
+    and then fix things up in recovery *)
+    result_rel rel (Crashed sigma1) (Crashed sigma2)
+| Failed_rel : result_rel rel Failed Failed.
+
+Hint Constructors Prog.exec.
+Hint Constructors result_rel.
+
+Ltac prog_bind :=
+  eapply Prog.ExecBindFinished.
+Ltac prog_step :=
+  first [ eapply Prog.ExecStepTo ||
+                 eapply Prog.ExecStepFail ];
+  simpl; simpl_match; eauto.
+
+Theorem translate_exec : forall T (p: seq_prog T),
+    forall ssigma sr,
+      exec p ssigma sr -> forall sigma,
+        sigma_rel ssigma sigma ->
+        exists r, Prog.exec (translate p) sigma r /\
+             result_rel sigma_rel sr r.
+Proof.
+  induction 1; intros.
+  - destruct p; simpl in *;
+      destruct matches in *;
+      match goal with
+      | [ H: _ = StepTo _ _ |- _ ] =>
+        inversion H; subst; clear H
+      end.
+    + exists (Finished v sigma0); intuition.
+      specialize (H0 a); simpl_match;
+        repeat deex.
+      unfold RRead_impl.
+      repeat (prog_bind; [ prog_step | ]); eauto.
+    + pose proof (H0 a); simpl_match;
+        repeat deex.
+      destruct sigma0; simpl in *; subst.
+      refine (ex_intro _ (Finished _ _) _); split.
+      repeat (prog_bind; [ prog_step | ]).
+      prog_step.
+
+      constructor.
+      unfold sigma_rel; intros; simpl.
+      destruct (is_eq a a0); subst;
+        autorewrite with upd.
+      descend; intuition eauto.
+      rewrite vote_eq; auto.
+      specialize (H0 a0).
+      destruct (sdisk sigma a0);
+        simpl in *; repeat deex.
+      descend; intuition eauto.
+      intuition.
+    + exists (Finished v sigma0); intuition.
+  - destruct p; simpl in *;
+      destruct matches in *;
+      match goal with
+      | [ H: _ = Fails |- _ ] =>
+        inversion H; subst; clear H
+      end.
+    exists Failed; intuition.
+    specialize (H0 a); simpl_match; intuition.
+    unfold RRead_impl.
+    eapply Prog.ExecBindFailed; prog_step.
+
+    exists Failed; intuition.
+    specialize (H0 a); simpl_match; intuition.
+    unfold RRead_impl.
+    eapply Prog.ExecBindFailed; prog_step.
+
+  - destruct p; simpl in *;
+      destruct matches in *;
+      match goal with
+      | [ H: _ = StepTo _ _ |- _ ] =>
+        inversion H; subst; clear H
+      end.
+    + exists (Crashed sigma0); intuition.
+    + pose proof (H0 a); simpl_match;
+        repeat deex.
+      destruct sigma0; simpl in *; subst.
+      refine (ex_intro _ (Crashed _) _); split.
+      repeat (prog_bind; [ prog_step | ]).
+      eapply Prog.ExecCrashAfter; simpl; simpl_match; eauto.
+
+      constructor.
+      unfold sigma_rel; intros; simpl.
+      destruct (is_eq a a0); subst;
+        autorewrite with upd.
+      descend; intuition eauto.
+      rewrite vote_eq; auto.
+      specialize (H0 a0).
+      destruct (sdisk sigma a0);
+        simpl in *; repeat deex.
+      descend; intuition eauto.
+      intuition.
+    + descend; intuition eauto.
+  - specialize (IHexec1 _ ltac:(eauto)); repeat deex.
+    match goal with
+    | [ H: result_rel sigma_rel  _ _ |- _ ] =>
+      inversion H; subst; clear H
+    end.
+    specialize (IHexec2 _ ltac:(eauto)); repeat deex.
+    simpl.
+    exists r0; intuition eauto.
+  - exists (Crashed sigma0); intuition eauto.
+  - specialize (IHexec _ ltac:(eauto)); repeat deex.
+    simpl.
+    match goal with
+    | [ H: result_rel sigma_rel  _ _ |- _ ] =>
+      inversion H; subst; clear H
+    end.
+    exists (Crashed sigma2); intuition eauto.
+  - specialize (IHexec _ ltac:(eauto)); repeat deex.
+    simpl.
+    match goal with
+    | [ H: result_rel sigma_rel  _ _ |- _ ] =>
+      inversion H; subst; clear H
+    end.
+    exists Failed; intuition eauto.
+Qed.
